examples/Msi.v
@@ -4,6 +4,7 @@ Set Implicit Arguments.
 
 Definition Msi := Bit 2.
 Definition Mod := 3.
+Definition Ex := 2.
 Definition Sh := 1.
 Definition Inv := 0.
 
@@ -13,9 +14,11 @@ Section HelperFunctions.
   Definition toCompat (x: Msi @ var): Msi @ var :=
     (IF (x == $ Mod)
      then $ Inv
-     else (IF (x == $ Sh)
+     else (IF (x == $ Ex)
            then $ Sh
-           else $ Mod))%kami_expr.
+           else (IF (x == $ Sh)
+                 then $ Ex
+                 else $ Mod)))%kami_expr.
 
   Definition isCompat (x y: Msi @ var) := (x <= toCompat y)%kami_expr.
 End HelperFunctions.
